Some more progress on idp refactoring

Protocol/Saml.fst
@@ -3,13 +3,45 @@ module Saml
 open Protocol
 open Network
 
+type Assertion = string
+type AuthnRequest = string
+type Response = string
 
 type SamlStatus =
   | Success: SamlStatus
   | Requester: SamlStatus
   | Responder: SamlStatus
 
-(*Saml functions*)
+type Samlmessage = 
+  | SamlAuthnRequestMessage: AuthnRequest -> dsig -> Samlmessage
+  | SamlResponseMessage: Response -> Samlmessage
+  | SamlStatusResponseMessage: SamlStatus -> Samlmessage
+
+
+(*Abstract saml methods*)
+val CreateAuthnRequest: issuer:prin -> destination:prin -> AuthnRequest
+val IssueSamlAssertion: idp:prin -> privkey idp -> AuthnRequest-> Subject ->  sp:prin -> pubkey sp ->  Assertion
+val CreateSamlResponse: prin -> AuthnRequest -> Assertion -> Samlmessage
+val CreateSamlFailedResponse: issuer:prin -> destination:prin -> SamlStatus -> Samlmessage
+
+(*Helper functions*)
+val IsAuthnRequest: list (string*string) -> bool
+val GetSamlMessage: list (string*string) -> (AuthnRequest * dsig)
+val CreateChallengeMessage: prin -> nonce -> Response
+
+val CreateRedirectResponse: prin -> Samlmessage -> HttpMessage
+let CreateRedirectResponse prin msg =
+      (*Base64 encode all params*)
+      match msg with 
+      | SamlAuthnRequestMessage (authReq, sig) ->
+      let params = [("samlmessage",authReq); ("signature",sig)] in
+      let cookies = [] in
+      let resp = Redirect prin prin params cookies in 
+      resp
+
+
+
+(*Saml functions
 extern reference Saml {language="F#";
             dll="Saml";
             namespace="";
@@ -19,11 +51,4 @@ extern Saml val CreateAuthnRequest: issuer:prin -> destination:prin -> samlmessa
 extern Saml val CreateSamlAssertion: user:string -> issuer:prin -> destination:prin -> assertion
 extern Saml val CreateSamlResponse: issuer:prin -> destination:prin -> assertion -> samlmessage
 extern Saml val CreateSamlFailedResponse: issuer:prin -> destination:prin -> SamlStatus -> samlmessage
-
-val CreateRedirectResponse: prin -> samlmessage -> dsig -> HttpMessage
-let CreateRedirectResponse prin msg sig =
-      (*Base64 encode all params*)
-      let params = [("samlmessage",msg); ("signature",sig)] in
-      let cookies = [] in
-      let resp = Redirect prin prin params cookies in 
-      resp
+*)
